<?xml version="1.0"?>

<!DOCTYPE rdf:RDF [
    <!ENTITY owl "http://www.w3.org/2002/07/owl#" >
    <!ENTITY obo "http://purl.obolibrary.org/obo/" >
    <!ENTITY xsd "http://www.w3.org/2001/XMLSchema#" >
    <!ENTITY rdfs "http://www.w3.org/2000/01/rdf-schema#" >
    <!ENTITY rdf "http://www.w3.org/1999/02/22-rdf-syntax-ns#" >
]>


<rdf:RDF xmlns="&obo;ro_imports.owl#"
     xml:base="&obo;ro_imports.owl"
     xmlns:obo="http://purl.obolibrary.org/obo/"
     xmlns:rdfs="http://www.w3.org/2000/01/rdf-schema#"
     xmlns:owl="http://www.w3.org/2002/07/owl#"
     xmlns:xsd="http://www.w3.org/2001/XMLSchema#"
     xmlns:rdf="http://www.w3.org/1999/02/22-rdf-syntax-ns#">
    <owl:Ontology rdf:about="http://purl.obolibrary.org/obo/caro/dev/ro_imports.owl">
    
    </owl:Ontology>
    
        
    
     <!-- http://purl.obolibrary.org/obo/RO_0002215 -->

    <owl:ObjectProperty rdf:about="&obo;RO_0002215">
        <rdfs:label xml:lang="en">capable of</rdfs:label>
        <obo:IAO_0000115>A relation between a material entity (such as a cell) and a process. This is a shortcut relation, translation rule for which is: capable_of P &lt;-&gt; bearer_of (some realized_by only P). Example: osteoclast capable of bone resorption.</obo:IAO_0000115>
        <obo:IAO_0000424>BFO_0000053 some (BFO_0000054 only ?Y)</obo:IAO_0000424>
        <obo:IAO_0000119>PMID:20123131</obo:IAO_0000119>
        <obo:IAO_0000117>Chris Mungall</obo:IAO_0000117>
        <obo:IAO_0000112>osteoclast SubClassOf &#39;capable of&#39; some &#39;bone resorption&#39;</obo:IAO_0000112>
        <obo:IAO_0000118>has function realized in</obo:IAO_0000118>
        <obo:IAO_0000119>PMID:21208450</obo:IAO_0000119>
        <rdfs:domain rdf:resource="&obo;BFO_0000004"/>
        <rdfs:range rdf:resource="&obo;BFO_0000015"/>
        <obo:IAO_0000114 rdf:resource="&obo;IAO_0000125"/>
        <owl:propertyChainAxiom rdf:parseType="Collection">
            <rdf:Description rdf:about="&obo;RO_0002214"/>
            <rdf:Description rdf:about="&obo;RO_0002217"/>
        </owl:propertyChainAxiom>
    </owl:ObjectProperty>
    

    <!-- http://purl.obolibrary.org/obo/RO_0002131 -->

    <owl:ObjectProperty rdf:about="&obo;RO_0002131">
        <rdfs:label xml:lang="en">overlaps</rdfs:label>
        <obo:IAO_0000424>http://purl.obolibrary.org/obo/BFO_0000051 some (http://purl.obolibrary.org/obo/BFO_0000050 some ?Y)</obo:IAO_0000424>
        <obo:IAO_0000115>x overlaps y if and only if there exists some z such that x has part z and z part of y</obo:IAO_0000115>
        <obo:IAO_0000114 rdf:resource="&obo;IAO_0000125"/>
        <rdfs:subPropertyOf rdf:resource="&owl;topObjectProperty"/>
        <owl:propertyChainAxiom rdf:parseType="Collection">
            <rdf:Description rdf:about="&obo;RO_0002131"/>
            <rdf:Description rdf:about="&obo;BFO_0000050"/>
        </owl:propertyChainAxiom>
        <owl:propertyChainAxiom rdf:parseType="Collection">
            <rdf:Description rdf:about="&obo;BFO_0000051"/>
            <rdf:Description rdf:about="&obo;RO_0002131"/>
        </owl:propertyChainAxiom>
        <owl:propertyChainAxiom rdf:parseType="Collection">
            <rdf:Description rdf:about="&obo;BFO_0000051"/>
            <rdf:Description rdf:about="&obo;BFO_0000050"/>
        </owl:propertyChainAxiom>
    </owl:ObjectProperty>
    
        <!-- http://purl.obolibrary.org/obo/RO_0002180 -->

    <owl:ObjectProperty rdf:about="&obo;RO_0002180">
        <rdfs:label xml:lang="en">has component</rdfs:label>
        <rdfs:comment xml:lang="en">For use in recording has_part with a cardinality constraint.</rdfs:comment>
        <rdfs:subPropertyOf rdf:resource="&obo;BFO_0000051"/>
        <obo:IAO_0000114 rdf:resource="&obo;IAO_0000125"/>
    </owl:ObjectProperty>
    
        <!-- http://purl.obolibrary.org/obo/BFO_0000050 -->

    <owl:ObjectProperty rdf:about="&obo;BFO_0000050">
        <rdf:type rdf:resource="&owl;TransitiveProperty"/>
        <rdfs:label xml:lang="en">part of</rdfs:label>
        <obo:IAO_0000412 rdf:resource="&obo;BFO"/>
        <owl:inverseOf rdf:resource="&obo;BFO_0000051"/>
        <rdfs:subPropertyOf rdf:resource="&obo;RO_0002131"/>
    </owl:ObjectProperty>
    


    <!-- http://purl.obolibrary.org/obo/BFO_0000051 -->

    <owl:ObjectProperty rdf:about="&obo;BFO_0000051">
        <rdf:type rdf:resource="&owl;TransitiveProperty"/>
        <rdfs:label xml:lang="en">has part</rdfs:label>
        <obo:IAO_0000412 rdf:resource="&obo;BFO"/>
        <rdfs:subPropertyOf rdf:resource="&obo;RO_0002131"/>
    </owl:ObjectProperty>
    
        <!-- http://purl.obolibrary.org/obo/RO_0002214 -->

    <owl:ObjectProperty rdf:about="&obo;RO_0002214">
        <rdfs:label xml:lang="en">has prototype</rdfs:label>
        <obo:IAO_0000112>&apos;human p53 protein&apos; SubClassOf some (&apos;participates in&apos; some &apos;DNA repair&apos;)</obo:IAO_0000112>
        <obo:IAO_0000117>Chris Mungall</obo:IAO_0000117>
        <obo:IAO_0000232>Experimental. In future there will be a formalization in which this relation is treated as a shortcut to some model logic axiom.</obo:IAO_0000232>
        <obo:IAO_0000112>heart SubClassOf &apos;has prototype&apos; some (&apos;participates in&apos; some &apos;blood circulation&apos;)</obo:IAO_0000112>
        <obo:IAO_0000115>x has prototype y if and only if x is an instance of C and y is a prototypical instance of C. For example, every instance of heart, both normal and abnormal is related by the has prototype relation to some instance of a &quot;canonical&quot; heart, which participates in blood circulation.</obo:IAO_0000115>
        <rdfs:range rdf:resource="&obo;BFO_0000002"/>
        <rdfs:domain rdf:resource="&obo;BFO_0000002"/>
        <obo:IAO_0000114 rdf:resource="&obo;IAO_0000125"/>
    </owl:ObjectProperty>
    
        <!-- http://purl.obolibrary.org/obo/RO_0002217 -->

    <owl:ObjectProperty rdf:about="&obo;RO_0002217">
        <rdfs:label xml:lang="en">actively participates in</rdfs:label>
        <obo:IAO_0000118>agent in</obo:IAO_0000118>
        <obo:IAO_0000115>x actively participates in y if and only if x participates in y and x realizes some active role</obo:IAO_0000115>
        <rdfs:subPropertyOf rdf:resource="&obo;BFO_0000056"/>
        <obo:IAO_0000114 rdf:resource="&obo;IAO_0000125"/>
        <owl:inverseOf rdf:resource="&obo;RO_0002218"/>
    </owl:ObjectProperty>
    
        <!-- http://purl.obolibrary.org/obo/RO_0002218 -->

    <owl:ObjectProperty rdf:about="&obo;RO_0002218">
        <rdfs:label xml:lang="en">has active participant</rdfs:label>
        <obo:IAO_0000118>has agent</obo:IAO_0000118>
        <obo:IAO_0000115>x has participant y if and only if x realizes some active role that inheres in y</obo:IAO_0000115>
        <rdfs:subPropertyOf rdf:resource="&obo;BFO_0000057"/>
        <obo:IAO_0000114 rdf:resource="&obo;IAO_0000125"/>
    </owl:ObjectProperty>
    
</rdf:RDF>    